Scratch, lift refactoring, maybe misguided

CpcMini/SmtModel.lean
@@ -587,7 +587,7 @@ def __vsm_apply_arg_nth : SmtValue -> native_Nat -> native_Nat -> SmtValue
 
 
 def __smtx_type_lift (s : native_String) (d : SmtDatatype) : SmtType -> SmtType
-  | (SmtType.Datatype s2 d2) => (native_ite (native_streq s s2) (SmtType.TypeRef s) (SmtType.Datatype s2 (__smtx_dt_lift s d d2)))
+  | (SmtType.Datatype s2 d2) => (native_ite (native_string_prefix_eq (native_string_lit "@") s2) (SmtType.Datatype s2 d2) (native_ite (native_streq s s2) (SmtType.TypeRef s) (SmtType.Datatype s2 (__smtx_dt_lift s d d2))))
   | T => T
 
 
